pm2.v
@@ -46,7 +46,7 @@ Proof.
     intros.
     pose (S1 := (comm (impl q r) (impl p q) (impl p r))).
     pose (S2 := (pm2_05 p q r)).
-    exact (pm1_11 S2 S1).
+    exact (mp S2 S1).
 Qed.
 
 Definition syll := pm2_06.
@@ -127,9 +127,9 @@ Theorem pm2_16 : forall (p q : Prop), (impl (impl p q) (impl (not q) (not p))).
 Proof.
     intros.
     pose (S1 := (pm2_12 q)).
-    pose (S2 := (pm1_11 S1 (pm2_05 p q (not (not q))))).
+    pose (S2 := (mp S1 (pm2_05 p q (not (not q))))).
     pose (S3 := (pm2_03 p (not q))).
-    exact (pm1_11 S3 (pm1_11 S2 (syll (impl p q) (impl p (not (not q))) (impl (not q) (not p))))).
+    exact (mp S3 (mp S2 (syll (impl p q) (impl p (not (not q))) (impl (not q) (not p))))).
 Qed.
 
 Definition transp0 := pm2_16.
@@ -139,8 +139,8 @@ Proof.
     intros.
     pose (S1 := (pm2_03 (not q) p)).
     pose (S2 := (pm2_14 q)).
-    pose (S3 := (pm1_11 S2 (pm2_05 p (not (not q)) q))).
-    exact (pm1_11 S3 (pm1_11 S1 (syll (impl (not q) (not p)) (impl p (not (not q))) (impl p q)))).
+    pose (S3 := (mp S2 (pm2_05 p (not (not q)) q))).
+    exact (mp S3 (mp S1 (syll (impl (not q) (not p)) (impl p (not (not q))) (impl p q)))).
 Qed.
 
 Definition transp3 := pm2_17.
@@ -149,11 +149,11 @@ Theorem pm2_18 : forall (p : Prop), (impl (impl (not p) p) p).
 Proof.
     intros.
     pose (S1 := (pm2_12 p)).
-    pose (S2 := (pm1_11 S1 (pm2_05 (not p) p (not (not p))))).
+    pose (S2 := (mp S1 (pm2_05 (not p) p (not (not p))))).
     pose (S3 := (pm2_01 (not p))).
-    pose (S4 := (pm1_11 S3 (pm1_11 S2 (syll (impl (not p) p) (impl (not p) (not (not p))) (not (not p)))))).
+    pose (S4 := (mp S3 (mp S2 (syll (impl (not p) p) (impl (not p) (not (not p))) (not (not p)))))).
     pose (S5 := (pm2_14 p)).
-    exact (pm1_11 S5 (pm1_11 S4 (syll (impl (not p) p) (not (not p)) p))).
+    exact (mp S5 (mp S4 (syll (impl (not p) p) (not (not p)) p))).
 Qed.
 
 Theorem pm2_2 : forall (p q : Prop), (impl p (or p q)).
@@ -161,7 +161,7 @@ Proof.
     intros.
     pose (S1 := (add q p)).
     pose (S2 := (perm q p)).
-    exact (pm1_11 S2 (pm1_11 S1 (syll p (or q p) (or p q)))).
+    exact (mp S2 (mp S1 (syll p (or q p) (or p q)))).
 Qed.
 
 Theorem pm2_21 : forall (p q : Prop), (impl (not p) (impl p q)).
@@ -173,14 +173,14 @@ Qed.
 Theorem pm2_24 : forall (p q : Prop), (impl p (impl (not p) q)).
 Proof.
     intros.
-    exact (pm1_11 (pm2_21 p q) (comm (not p) p q)).
+    exact (mp (pm2_21 p q) (comm (not p) p q)).
 Qed.
 
 Theorem pm2_25 : forall (p q : Prop), (or p (impl (or p q) q)).
 Proof.
     intros.
     pose (S1 := (pm2_1 (or p q))).
-    exact (pm1_11 S1 (pm1_5 (not (or p q)) p q)).
+    exact (mp S1 (pm1_5 (not (or p q)) p q)).
 Qed.
 
 Theorem pm2_26 : forall (p q : Prop), (or (not p) (impl (impl p q) q)).
@@ -199,7 +199,7 @@ Theorem pm2_3 : forall (p q r : Prop), (impl (or p (or q r)) (or p (or r q))).
 Proof.
     intros.
     pose (S1 := (perm q r)).
-    exact (pm1_11 S1 (sum p (or q r) (or r q))).
+    exact (mp S1 (sum p (or q r) (or r q))).
 Qed.
 
 Theorem pm2_31 : forall (p q r : Prop), (impl (or p (or q r)) (or (or p q) r)).
@@ -214,8 +214,8 @@ Theorem pm2_32 : forall (p q r : Prop), (impl (or (or p q) r) (or p (or q r))).
 Proof.
     intros.
     pose (S1 := (perm (or p q) r)).
-    pose (S2 := (pm1_11 (assoc r p q) (pm1_11 S1 (syll (or (or p q) r) (or r (or p q)) (or p (or r q)))))).
-    exact (pm1_11 (pm2_3 p r q) (pm1_11 S2 (syll (or (or p q) r) (or p (or r q)) (or p (or q r))))).
+    pose (S2 := (mp (assoc r p q) (mp S1 (syll (or (or p q) r) (or r (or p q)) (or p (or r q)))))).
+    exact (mp (pm2_3 p r q) (mp S2 (syll (or (or p q) r) (or p (or r q)) (or p (or q r))))).
 Qed.
 
 Definition or3 := fun (p q r : Prop) => (or (or p q) r).
@@ -224,41 +224,41 @@ Theorem pm2_36 : forall (p q r : Prop), (impl (impl q r) (impl (or p q) (or r p)
 Proof.
     intros.
     pose (S1 := (perm p r)).
-    pose (S2 := (pm1_11 S1 (syllr (or p q) (or p r) (or r p)))).
+    pose (S2 := (mp S1 (syllr (or p q) (or p r) (or r p)))).
     pose (S3 := (sum p q r)).
-    exact (pm1_11 S2 (pm1_11 S3 (syll (impl q r) (impl (or p q) (or p r)) (impl (or p q) (or r p))))).
+    exact (mp S2 (mp S3 (syll (impl q r) (impl (or p q) (or p r)) (impl (or p q) (or r p))))).
 Qed.
 
 Theorem pm2_37 : forall (p q r : Prop), (impl (impl q r) (impl (or q p) (or p r))).
 Proof.
     intros.
     pose (S1 := (perm q p)).
-    pose (S2 := (pm1_11 S1 (syll (or q p) (or p q) (or p r)))).
+    pose (S2 := (mp S1 (syll (or q p) (or p q) (or p r)))).
     pose (S3 := (sum p q r)).
-    exact (pm1_11 S2 (pm1_11 S3 (syll (impl q r) (impl (or p q) (or p r)) (impl (or q p) (or p r))))).
+    exact (mp S2 (mp S3 (syll (impl q r) (impl (or p q) (or p r)) (impl (or q p) (or p r))))).
 Qed.
 
 Theorem pm2_38 : forall (p q r : Prop), (impl (impl q r) (impl (or q p) (or r p))).
 Proof.
     intros.
     pose (S1 := (perm q p)).
-    pose (S2 := (pm1_11 S1 (syll (or q p) (or p q) (or r p)))).
+    pose (S2 := (mp S1 (syll (or q p) (or p q) (or r p)))).
     pose (S3 := (pm2_36 p q r)).
-    exact (pm1_11 S2 (pm1_11 S3 (syll (impl q r) (impl (or p q) (or r p)) (impl (or q p) (or r p))))).
+    exact (mp S2 (mp S3 (syll (impl q r) (impl (or p q) (or r p)) (impl (or q p) (or r p))))).
 Qed.
 
 Theorem pm2_4 : forall (p q : Prop), (impl (or p (or p q)) (or p q)).
 Proof.
     intros.
     pose (S1 := (pm2_31 p p q)).
-    exact (pm1_11 (pm1_11 (taut p) (pm2_38 q (or p p) p)) (pm1_11 S1 (syll (or p (or p q)) (or (or p p) q) (or p q)))).
+    exact (mp (mp (taut p) (pm2_38 q (or p p) p)) (mp S1 (syll (or p (or p q)) (or (or p p) q) (or p q)))).
 Qed.
 
 Theorem pm2_41 : forall (p q : Prop), (impl (or q (or p q)) (or p q)).
 Proof.
     intros.
     pose (S1 := (assoc q p q)).
-    exact (pm1_11 (pm1_11 (taut q) (sum p (or q q) q)) (pm1_11 S1 (syll (or q (or p q)) (or p (or q q)) (or p q)))).
+    exact (mp (mp (taut q) (sum p (or q q) q)) (mp S1 (syll (or q (or p q)) (or p (or q q)) (or p q)))).
 Qed.
 
 Theorem pm2_42 : forall (p q : Prop), (impl (or (not p) (impl p q)) (impl p q)).
@@ -276,31 +276,31 @@ Qed.
 Theorem pm2_45 : forall (p q : Prop), (impl (not (or p q)) (not p)).
 Proof.
     intros.
-    exact (pm1_11 (pm2_2 p q) (transp0 p (or p q))).
+    exact (mp (pm2_2 p q) (transp0 p (or p q))).
 Qed.
 
 Theorem pm2_46 : forall (p q : Prop), (impl (not (or p q)) (not q)).
 Proof.
     intros.
-    exact (pm1_11 (pm1_3 p q) (transp0 q (or p q))).
+    exact (mp (pm1_3 p q) (transp0 q (or p q))).
 Qed.
 
 Theorem pm2_47 : forall (p q : Prop), (impl (not (or p q)) (or (not p) q)).
 Proof.
     intros.
-    exact (pm1_11 (pm2_2 (not p) q) (pm1_11 (pm2_45 p q) (syll (not (or p q)) (not p) (or (not p) q)))).
+    exact (mp (pm2_2 (not p) q) (mp (pm2_45 p q) (syll (not (or p q)) (not p) (or (not p) q)))).
 Qed.
 
 Theorem pm2_48 : forall (p q : Prop), (impl (not (or p q)) (or p (not q))).
 Proof.
     intros.
-    exact (pm1_11 (pm1_3 p (not q)) (pm1_11 (pm2_46 p q) (syll (not (or p q)) (not q) (or p (not q))))).
+    exact (mp (pm1_3 p (not q)) (mp (pm2_46 p q) (syll (not (or p q)) (not q) (or p (not q))))).
 Qed.
 
 Theorem pm2_49 : forall (p q : Prop), (impl (not (or p q)) (or (not p) (not q))).
 Proof.
     intros.
-    exact (pm1_11 (pm2_2 (not p) (not q)) (pm1_11 (pm2_45 p q) (syll (not (or p q)) (not p) (or (not p) (not q))))).
+    exact (mp (pm2_2 (not p) (not q)) (mp (pm2_45 p q) (syll (not (or p q)) (not p) (or (not p) (not q))))).
 Qed.
 
 Theorem pm2_5 : forall (p q : Prop), (impl (not (impl p q)) (impl (not p) q)).
@@ -324,57 +324,57 @@ Qed.
 Theorem pm2_521 : forall (p q : Prop), (impl (not (impl p q)) (impl q p)).
 Proof.
     intros.
-    exact (pm1_11 (pm2_17 q p) (pm1_11 (pm2_52 p q) (syll (not (impl p q)) (impl (not p) (not q)) (impl q p)))).
+    exact (mp (pm2_17 q p) (mp (pm2_52 p q) (syll (not (impl p q)) (impl (not p) (not q)) (impl q p)))).
 Qed.
 
 Theorem pm2_53 : forall (p q : Prop), (impl (or p q) (impl (not p) q)).
 Proof.
     intros.
-    exact (pm1_11 (pm2_12 p) (pm2_38 q p (not (not p)))).
+    exact (mp (pm2_12 p) (pm2_38 q p (not (not p)))).
 Qed.
 
 Theorem pm2_54 : forall (p q : Prop), (impl (impl (not p) q) (or p q)).
 Proof.
     intros.
-    exact (pm1_11 (pm2_14 p) (pm2_38 q (not (not p)) p)).
+    exact (mp (pm2_14 p) (pm2_38 q (not (not p)) p)).
 Qed.
 
 Theorem pm2_55 : forall (p q : Prop), (impl (not p) (impl (or p q) q)).
 Proof.
     intros.
-    exact (pm1_11 (pm2_53 p q) (comm (or p q) (not p) q)).
+    exact (mp (pm2_53 p q) (comm (or p q) (not p) q)).
 Qed.
 
 Theorem pm2_56 : forall (p q : Prop), (impl (not q) (impl (or p q) p)).
 Proof.
     intros.
-    exact (pm1_11 (pm1_11 (perm p q) (syll (or p q) (or q p) p)) (pm1_11 (pm2_55 q p) (syll (not q) (impl (or q p) p) (impl (or p q) p)))).
+    exact (mp (mp (perm p q) (syll (or p q) (or q p) p)) (mp (pm2_55 q p) (syll (not q) (impl (or q p) p) (impl (or p q) p)))).
 Qed.
 
 Theorem pm2_6 : forall (p q : Prop), (impl (impl (not p) q) (impl (impl p q) q)).
 Proof.
     intros.
     pose (S1 := (pm2_38 q (not p) q)).
-    pose (S2 := (pm1_11 (taut q) (syllr (or (not p) q) (or q q) q))).
-    exact (pm1_11 S2 (pm1_11 S1 (syll (impl (not p) q) (impl (or (not p) q) (or q q)) (impl (or (not p) q) q)))).
+    pose (S2 := (mp (taut q) (syllr (or (not p) q) (or q q) q))).
+    exact (mp S2 (mp S1 (syll (impl (not p) q) (impl (or (not p) q) (or q q)) (impl (or (not p) q) q)))).
 Qed.
 
 Theorem pm2_61 : forall (p q : Prop), (impl (impl p q) (impl (impl (not p) q) q)).
 Proof.
     intros.
-    exact (pm1_11 (pm2_6 p q) (comm (impl (not p) q) (impl p q) q)).
+    exact (mp (pm2_6 p q) (comm (impl (not p) q) (impl p q) q)).
 Qed.
 
 Theorem pm2_62 : forall (p q : Prop), (impl (or p q) (impl (impl p q) q)).
 Proof.
     intros.
-    exact (pm1_11 (pm2_6 p q) (pm1_11 (pm2_53 p q) (syll (or p q) (impl (not p) q) (impl (impl p q) q)))).
+    exact (mp (pm2_6 p q) (mp (pm2_53 p q) (syll (or p q) (impl (not p) q) (impl (impl p q) q)))).
 Qed.
 
 Theorem pm2_621 : forall (p q : Prop), (impl (impl p q) (impl (or p q) q)).
 Proof.
     intros.
-    exact (pm1_11 (pm2_62 p q) (comm (or p q) (impl p q) q)).
+    exact (mp (pm2_62 p q) (comm (or p q) (impl p q) q)).
 Qed.
 
 Theorem pm2_63 : forall (p q : Prop), (impl (or p q) (impl (or (not p) q) q)).
@@ -386,7 +386,7 @@ Qed.
 Theorem pm2_64 : forall (p q : Prop), (impl (or p q) (impl (or p (not q)) p)).
 Proof.
     intros.
-    exact (pm1_11 (pm1_11 (pm1_11 (perm p (not q)) (syll (or p (not q)) (or (not q) p) p)) (pm1_11 (pm2_63 q p) (syll (or q p) (impl (or (not q) p) p) (impl (or p (not q)) p)))) (pm1_11 (perm p q) (syll (or p q) (or q p) (impl (or p (not q)) p)))).
+    exact (mp (mp (mp (perm p (not q)) (syll (or p (not q)) (or (not q) p) p)) (mp (pm2_63 q p) (syll (or q p) (impl (or (not q) p) p) (impl (or p (not q)) p)))) (mp (perm p q) (syll (or p q) (or q p) (impl (or p (not q)) p)))).
 Qed.
 
 Theorem pm2_65 : forall (p q : Prop), (impl (impl p q) (impl (impl p (not q)) (not p))).
@@ -398,46 +398,46 @@ Qed.
 Theorem pm2_67 : forall (p q : Prop), (impl (impl (or p q) q) (impl p q)).
 Proof.
     intros.
-    pose (S1 := (pm1_11 (pm2_54 p q) (syll (impl (not p) q) (or p q) q))).
-    pose (S2 := (pm1_11 (pm2_24 p q) (syll p (impl (not p) q) q))).
-    exact (pm1_11 S2 (pm1_11 S1 (syll (impl (or p q) q) (impl (impl (not p) q) q) (impl p q)))).
+    pose (S1 := (mp (pm2_54 p q) (syll (impl (not p) q) (or p q) q))).
+    pose (S2 := (mp (pm2_24 p q) (syll p (impl (not p) q) q))).
+    exact (mp S2 (mp S1 (syll (impl (or p q) q) (impl (impl (not p) q) q) (impl p q)))).
 Qed.
 
 Theorem pm2_68 : forall (p q : Prop), (impl (impl (impl p q) q) (or p q)).
 Proof.
     intros.
     pose (S1 := (pm2_67 (not p) q)).
-    exact (pm1_11 (pm2_54 p q) (pm1_11 S1 (syll (impl (impl p q) q) (impl (not p) q) (or p q)))).
+    exact (mp (pm2_54 p q) (mp S1 (syll (impl (impl p q) q) (impl (not p) q) (or p q)))).
 Qed.
 
 Theorem pm2_69 : forall (p q : Prop), (impl (impl (impl p q) q) (impl (impl q p) p)).
 Proof.
     intros.
-    exact (pm1_11 (pm2_62 q p) (pm1_11 (pm1_11 (perm p q) (pm1_11 (pm2_68 p q) (syll (impl (impl p q) q) (or p q) (or q p)))) (syll (impl (impl p q) q) (or q p) (impl (impl q p) p)))).
+    exact (mp (pm2_62 q p) (mp (mp (perm p q) (mp (pm2_68 p q) (syll (impl (impl p q) q) (or p q) (or q p)))) (syll (impl (impl p q) q) (or q p) (impl (impl q p) p)))).
 Qed.
 
 Theorem pm2_73 : forall (p q r : Prop), (impl (impl p q) (impl (or3 p q r) (or q r))).
 Proof.
     intros.
-    exact (pm1_11 (pm2_38 r (or p q) q) (pm1_11 (pm2_621 p q) (syll (impl p q) (impl (or p q) q) (impl (or3 p q r) (or q r))))).
+    exact (mp (pm2_38 r (or p q) q) (mp (pm2_621 p q) (syll (impl p q) (impl (or p q) q) (impl (or3 p q r) (or q r))))).
 Qed.
 
 Theorem pm2_74 : forall (p q r : Prop), (impl (impl q p) (impl (or3 p q r) (or p r))).
 Proof.
     intros.
-    exact (pm1_11 (pm1_11 (pm1_11 (perm p q) (pm2_38 r (or p q) (or q p))) (syll (or3 p q r) (or3 q p r) (or p r))) (pm1_11 (pm2_73 q p r) (syll (impl q p) (impl (or3 q p r) (or p r)) (impl (or3 p q r) (or p r))))).
+    exact (mp (mp (mp (perm p q) (pm2_38 r (or p q) (or q p))) (syll (or3 p q r) (or3 q p r) (or p r))) (mp (pm2_73 q p r) (syll (impl q p) (impl (or3 q p r) (or p r)) (impl (or3 p q r) (or p r))))).
 Qed.
 
 Theorem pm2_75 : forall (p q r : Prop), (impl (or p q) (impl (or p (impl q r)) (or p r))).
 Proof.
     intros.
-    exact (pm1_11 (pm1_11 (pm2_31 p (not q) r) (syll (or p (impl q r)) (or3 p (not q) r) (or p r))) (pm1_11 (pm1_11 (pm1_11 (pm2_74 p (not q) r) (pm1_11 (pm2_53 q p) (syll (or q p) (impl (not q) p) (impl (or3 p (not q) r) (or p r))))) (pm1_11 (perm p q) (syll (or p q) (or q p) (impl (or3 p (not q) r) (or p r))))) (syll (or p q) (impl (or3 p (not q) r) (or p r)) (impl (or p (impl q r)) (or p r))))).
+    exact (mp (mp (pm2_31 p (not q) r) (syll (or p (impl q r)) (or3 p (not q) r) (or p r))) (mp (mp (mp (pm2_74 p (not q) r) (mp (pm2_53 q p) (syll (or q p) (impl (not q) p) (impl (or3 p (not q) r) (or p r))))) (mp (perm p q) (syll (or p q) (or q p) (impl (or3 p (not q) r) (or p r))))) (syll (or p q) (impl (or3 p (not q) r) (or p r)) (impl (or p (impl q r)) (or p r))))).
 Qed.
 
 Theorem pm2_76 : forall (p q r : Prop), (impl (or p (impl q r)) (impl (or p q) (or p r))).
 Proof.
     intros.
-    exact (pm1_11 (pm2_75 p q r) (comm (or p q) (or p (impl q r)) (or p r))).
+    exact (mp (pm2_75 p q r) (comm (or p q) (or p (impl q r)) (or p r))).
 Qed.
 
 Theorem pm2_77 : forall (p q r : Prop), (impl (impl p (impl q r)) (impl (impl p q) (impl p r))).
@@ -449,39 +449,39 @@ Qed.
 Theorem pm2_8 : forall (q r s : Prop), (impl (or q r) (impl (or (not r) s) (or q s))).
 Proof.
     intros.
-    pose (S1 := (pm1_11 (pm2_53 r q) (pm1_11 (perm q r) (syll (or q r) (or r q) (impl (not r) q))))).
-    exact (pm1_11 (pm2_38 s (not r) q) (pm1_11 S1 (syll (or q r) (impl (not r) q) (impl (or (not r) s) (or q s))))).
+    pose (S1 := (mp (pm2_53 r q) (mp (perm q r) (syll (or q r) (or r q) (impl (not r) q))))).
+    exact (mp (pm2_38 s (not r) q) (mp S1 (syll (or q r) (impl (not r) q) (impl (or (not r) s) (or q s))))).
 Qed.
 
 Theorem pm2_81 : forall (p q r s : Prop), (impl (impl q (impl r s)) (impl (or p q) (impl (or p r) (or p s)))).
 Proof.
     intros.
     pose (S1 := (sum p q (impl r s))).
-    pose (S2 := (pm1_11 (pm2_76 p r s) (syllr (or p q) (or p (impl r s)) (impl (or p r) (or p s))))).
-    exact (pm1_11 S2 (pm1_11 S1 (syll (impl q (impl r s)) (impl (or p q) (or p (impl r s))) (impl (or p q) (impl (or p r) (or p s)))))).
+    pose (S2 := (mp (pm2_76 p r s) (syllr (or p q) (or p (impl r s)) (impl (or p r) (or p s))))).
+    exact (mp S2 (mp S1 (syll (impl q (impl r s)) (impl (or p q) (or p (impl r s))) (impl (or p q) (impl (or p r) (or p s)))))).
 Qed.
 
 Theorem pm2_82 : forall (p q r s : Prop), (impl (or3 p q r) (impl (or3 p (not r) s) (or3 p q s))).
 Proof.
     intros.
-    exact (pm1_11 (pm1_11 (pm1_11 (pm1_11 (pm2_32 p (not r) s) (syll (or3 p (not r) s) (or p (or (not r) s)) (or3 p q s))) (pm1_11 (pm1_11 (pm2_31 p q s) (syllr (or p (or (not r) s)) (or p (or q s)) (or3 p q s))) (syll (impl (or p (or (not r) s)) (or p (or q s))) (impl (or p (or (not r) s)) (or3 p q s)) (impl (or3 p (not r) s) (or3 p q s))))) (pm1_11 (pm1_11 (pm2_8 q r s) (pm2_81 p (or q r) (or (not r) s) (or q s))) (syll (or p (or q r)) (impl (or p (or (not r) s)) (or p (or q s))) (impl (or3 p (not r) s) (or3 p q s))))) (pm1_11 (pm2_32 p q r) (syll (or3 p q r) (or p (or q r)) (impl (or3 p (not r) s) (or3 p q s))))).
+    exact (mp (mp (mp (mp (pm2_32 p (not r) s) (syll (or3 p (not r) s) (or p (or (not r) s)) (or3 p q s))) (mp (mp (pm2_31 p q s) (syllr (or p (or (not r) s)) (or p (or q s)) (or3 p q s))) (syll (impl (or p (or (not r) s)) (or p (or q s))) (impl (or p (or (not r) s)) (or3 p q s)) (impl (or3 p (not r) s) (or3 p q s))))) (mp (mp (pm2_8 q r s) (pm2_81 p (or q r) (or (not r) s) (or q s))) (syll (or p (or q r)) (impl (or p (or (not r) s)) (or p (or q s))) (impl (or3 p (not r) s) (or3 p q s))))) (mp (pm2_32 p q r) (syll (or3 p q r) (or p (or q r)) (impl (or3 p (not r) s) (or3 p q s))))).
 Qed.
 
 Theorem pm2_83 : forall (p q r s : Prop), (impl (impl p (impl q r)) (impl (impl p (impl r s)) (impl p (impl q s)))).
 Proof.
     intros.
-    exact (pm1_11 (pm1_11 (pm1_11 (pm1_11 (pm2_31 (not p) (not r) s) (syll (impl p (impl r s)) (or3 (not p) (not r) s) (impl p (impl q s)))) (pm1_11 (pm1_11 (pm2_32 (not p) (not q) s) (syllr (or3 (not p) (not r) s) (or3 (not p) (not q) s) (impl p (impl q s)))) (syll (impl (or3 (not p) (not r) s) (or3 (not p) (not q) s)) (impl (or3 (not p) (not r) s) (impl p (impl q s))) (impl (impl p (impl r s)) (impl p (impl q s)))))) (pm1_11 (pm2_82 (not p) (not q) r s) (syll (or3 (not p) (not q) r) (impl (or3 (not p) (not r) s) (or3 (not p) (not q) s)) (impl (impl p (impl r s)) (impl p (impl q s)))))) (pm1_11 (pm2_31 (not p) (not q) r) (syll (impl p (impl q r)) (or3 (not p) (not q) r) (impl (impl p (impl r s)) (impl p (impl q s)))))).
+    exact (mp (mp (mp (mp (pm2_31 (not p) (not r) s) (syll (impl p (impl r s)) (or3 (not p) (not r) s) (impl p (impl q s)))) (mp (mp (pm2_32 (not p) (not q) s) (syllr (or3 (not p) (not r) s) (or3 (not p) (not q) s) (impl p (impl q s)))) (syll (impl (or3 (not p) (not r) s) (or3 (not p) (not q) s)) (impl (or3 (not p) (not r) s) (impl p (impl q s))) (impl (impl p (impl r s)) (impl p (impl q s)))))) (mp (pm2_82 (not p) (not q) r s) (syll (or3 (not p) (not q) r) (impl (or3 (not p) (not r) s) (or3 (not p) (not q) s)) (impl (impl p (impl r s)) (impl p (impl q s)))))) (mp (pm2_31 (not p) (not q) r) (syll (impl p (impl q r)) (or3 (not p) (not q) r) (impl (impl p (impl r s)) (impl p (impl q s)))))).
 Qed.
 
 Theorem pm2_85 : forall (p q r : Prop), (impl (impl (or p q) (or p r)) (or p (impl q r))).
 Proof.
     intros.
-    pose (S1 := (pm1_11 (add p q) (syll q (or p q) r))).
+    pose (S1 := (mp (add p q) (syll q (or p q) r))).
     pose (S2 := (pm2_55 p r)).
-    pose (S3 := (pm1_11 (syllr (or p q) (or p r) r) (pm1_11 S2 (syll (not p) (impl (or p r) r) (impl (impl (or p q) (or p r)) (impl (or p q) r)))))).
-    pose (S4 := (pm1_11 (pm1_11 S1 (syllr (impl (or p q) (or p r)) (impl (or p q) r) (impl q r))) (pm1_11 S3 (syll (not p) (impl (impl (or p q) (or p r)) (impl (or p q) r)) (impl (impl (or p q) (or p r)) (impl q r)))))).
-    pose (S5 := (pm1_11 S4 (comm (not p) (impl (or p q) (or p r)) (impl q r)))).
-    exact (pm1_11 (pm2_54 p (impl q r)) (pm1_11 S5 (syll (impl (or p q) (or p r)) (impl (not p) (impl q r)) (or p (impl q r))))).
+    pose (S3 := (mp (syllr (or p q) (or p r) r) (mp S2 (syll (not p) (impl (or p r) r) (impl (impl (or p q) (or p r)) (impl (or p q) r)))))).
+    pose (S4 := (mp (mp S1 (syllr (impl (or p q) (or p r)) (impl (or p q) r) (impl q r))) (mp S3 (syll (not p) (impl (impl (or p q) (or p r)) (impl (or p q) r)) (impl (impl (or p q) (or p r)) (impl q r)))))).
+    pose (S5 := (mp S4 (comm (not p) (impl (or p q) (or p r)) (impl q r)))).
+    exact (mp (pm2_54 p (impl q r)) (mp S5 (syll (impl (or p q) (or p r)) (impl (not p) (impl q r)) (or p (impl q r))))).
 Qed.
 
 Theorem pm2_86 : forall (p q r : Prop), (impl (impl (impl p q) (impl p r)) (impl p (impl q r))).
